Solanalib.lean
@@ -17,8 +17,10 @@ import Solanalib.Primitives.Lamports
 import Solanalib.Primitives.Pubkey
 import Solanalib.Primitives.Time
 import Solanalib.SBPF.CommType
+import Solanalib.SBPF.Decoder
 import Solanalib.SBPF.Memory
 import Solanalib.SBPF.Syntax
+import Solanalib.SBPF.Value
 
 /-!
 # Solanalib
